examples/pick_left.v
@@ -3,68 +3,16 @@ Add LoadPath "C:\Users\Ziga\Documents\Ziga_podatki\repositories\eeff-formalizati
 Add LoadPath "C:\Users\Ziga\Documents\Ziga_podatki\repositories\eeff-formalization\substitution".
 Add LoadPath "C:\Users\Ziga\Documents\Ziga_podatki\repositories\eeff-formalization\operational_semantics".
 Add LoadPath "C:\Users\Ziga\Documents\Ziga_podatki\repositories\eeff-formalization\logic".
+Add LoadPath "C:\Users\Ziga\Documents\Ziga_podatki\repositories\eeff-formalization\examples".
 (* Add LoadPath "E:\Ziga_Podatki\faks\eeff-formalization\syntax". *)
 (* Add LoadPath "E:\Ziga_Podatki\faks\eeff-formalization\type_system". *)
 (* Add LoadPath "E:\Ziga_Podatki\faks\eeff-formalization\substitution". *)
 (* Add LoadPath "E:\Ziga_Podatki\faks\eeff-formalization\operational_semantics". *)
 (* Add LoadPath "E:\Ziga_Podatki\faks\eeff-formalization\logic". *)
+(* Add LoadPath "E:\Ziga_Podatki\faks\eeff-formalization\examples". *)
 
-Require Export type_lemmas logic_lemmas.
+Require Export type_lemmas logic_lemmas logic_tactics.
 Open Scope string_scope.
-
-Ltac simpl_c_subs := 
-  unfold c_subs2_out; unfold c_subs_out; unfold c_subs; simpl.
-
-Ltac obvious := 
-     apply WfCtxØ || (apply WfCtxU; obvious) 
-  || apply WfTCtxØ  || (apply WfTCtxU; obvious) 
-  || apply WfEqsØ || apply WfSigØ || (apply WfSigU; obvious)
-  || apply WfTyUnit || apply WfTyInt || (apply WfTyHandler; obvious)
-  || (apply WfTyFun; obvious) || (apply WfTyΣ; obvious)
-  || (apply WfTyΠ; obvious) || (apply WfCTy; obvious)
-  || auto.
-
-Ltac obvious_vtype := (
-  (apply TypeV; (
-     (apply TypeUnit; obvious)
-  || (apply TypeInt; obvious)
-  || (apply TypeInl; obvious_vtype)
-  || (apply TypeInr; obvious_vtype)
-  || (apply TypeVar; simpl in *; obvious)
-  || obvious)
-  )
-  || obvious).
-
-Ltac vtype_step := (
-  (apply TypeV; (
-     (apply TypeUnit; obvious)
-  || (apply TypeInt; obvious)
-  || (apply TypeInl; obvious)
-  || (apply TypeInr; obvious)
-  || (apply TypeFun; obvious)
-  || (apply TypeVar; simpl in *; obvious)
-  || obvious)
-  )
-  || obvious).
-
-
-Ltac obvious_ctype := (
-  (apply TypeC; (
-    (apply TypeRet; obvious_vtype)
- || (eapply TypeApp; obvious_vtype)
- || (eapply TypeΣMatch; obvious_vtype)
- || obvious)
- )
- || obvious).
-
-Ltac ctype_step := (
-  (apply TypeC; (
-    (apply TypeRet; obvious)
- || (eapply TypeApp; obvious)
- || (eapply TypeΣMatch; obvious)
- || obvious)
- )
- || obvious).
 
 (* ========================================================================== *)
 
